examples/technical_report/Isabelle_DOF-Manual/04_RefMan.thy
@@ -159,7 +159,7 @@ text\<open>
   to instances, and class-invariants. Some concepts like  advanced type-checking, referencing to 
   formal entities of Isabelle, and monitors are due to its specific application in the 
   Isabelle context. Conceptually, ontologies specified in ODL consist of:
-  \<^item> \<^emph>\<open>document classes\<close> (\inlineisar{doc_class}) that describe concepts;
+  \<^item> \<^emph>\<open>document classes\<close> (\<^boxed_theory_text>\<open>doc_class\<close>) that describe concepts;
   \<^item> an optional document base class expressing single inheritance
   class extensions;
   \<^item> \<^emph>\<open>attributes\<close> specific to document classes, where
@@ -192,15 +192,15 @@ text\<open>
 
 text\<open>
   Attributes referring to other ontological concepts are called \<^emph>\<open>links\<close>. The HOL-types inside the 
-  document specification language support built-in types for Isabelle/HOL \inlineisar+typ+'s,  
-  \inlineisar+term+'s, and \inlineisar+thm+'s reflecting internal Isabelle's  internal types for 
+  document specification language support built-in types for Isabelle/HOL \<^boxed_theory_text>\<open>typ\<close>'s,  
+  \<^boxed_theory_text>\<open>term\<close>'s, and \<^boxed_theory_text>\<open>thm\<close>'s reflecting internal Isabelle's  internal types for 
   these entities; when denoted in HOL-terms to instantiate an attribute, for example, there is a  
   specific syntax (called \<^emph>\<open>inner syntax antiquotations\<close>) that is checked by 
   \isadof for consistency.
 
   Document classes\bindex{document class}\index{class!document@see document class} support 
-  \inlineisar+where+-clauses\index{where clause} containing a regular expression over class 
-  names. Classes with a \inlineisar+where+ were called 
+  \<^boxed_theory_text>\<open>where\<close>-clauses\index{where clause} containing a regular expression over class 
+  names. Classes with a \<^boxed_theory_text>\<open>where\<close> were called 
   \<^emph>\<open>monitor classes\<close>.\bindex{monitor class}\index{class!monitor@see monitor class} While document 
   classes and their inheritance relation structure meta-data of text-elements in an object-oriented 
   manner, monitor classes enforce structural organization of documents via the language specified 
@@ -208,8 +208,8 @@ text\<open>
 
   A major design decision of ODL is to denote attribute values by HOL-terms and HOL-types. 
   Consequently, ODL can refer to any predefined type defined in the HOL library, \eg, 
-  \inlineisar+string+ or \inlineisar+int+ as well as parameterized types, \eg, \inlineisar+_ option+, 
-  \inlineisar+_ list+, \inlineisar+_ set+, or products \inlineisar+_ \<times> _+. As a consequence of the 
+  \<^boxed_theory_text>\<open>string\<close> or \<^boxed_theory_text>\<open>int\<close> as well as parameterized types, \eg, \<^boxed_theory_text>\<open>_ option\<close>, 
+  \<^boxed_theory_text>\<open>_ list\<close>, \<^boxed_theory_text>\<open>_ set\<close>, or products \<^boxed_theory_text>\<open>_ \<times> _\<close>. As a consequence of the 
   document model, ODL definitions may be arbitrarily intertwined with standard HOL type definitions. 
   Finally, document class definitions result in themselves in a HOL-types in order to allow \<^emph>\<open>links\<close> 
   to and between ontological concepts.
@@ -226,8 +226,8 @@ text\<open>
   \<^item> \<open>name\<close>:\index{name@\<open>name\<close>}
      with the syntactic category of \<open>name\<close>'s we refer to alpha-numerical identifiers 
      (called \<open>short_id\<close>'s in @{cite "wenzel:isabelle-isar:2020"}) and identifiers
-     in \inlineisar+" ... "+ which might contain certain ``quasi-letters'' such 
-     as \inlineisar+_+, \inlineisar+-+, \inlineisar+.+ (see~@{cite "wenzel:isabelle-isar:2020"} for 
+     in \<^boxed_theory_text>\<open> ... \<close> which might contain certain ``quasi-letters'' such 
+     as \<^boxed_theory_text>\<open>_\<close>, \<^boxed_theory_text>\<open>-\<close>, \<^boxed_theory_text>\<open>.\<close> (see~@{cite "wenzel:isabelle-isar:2020"} for 
      details).
   \<^item> \<open>tyargs\<close>:\index{tyargs@\<open>tyargs\<close>} 
      \<^rail>\<open>  typefree | ('(' (typefree * ',') ')')\<close>
@@ -242,7 +242,6 @@ text\<open>
      The \<open>name\<close>'s referred here are type names such as \<^verbatim>\<open>int\<close>, \<^verbatim>\<open>string\<close>, \<^verbatim>\<open>list\<close>, \<^verbatim>\<open>set\<close>, etc. 
   \<^item> \<open>type\<close>:\index{type@\<open>type\<close>}
      \<^rail>\<open>  (( '(' ( type * ',')  ')' )? name) | typefree \<close>     
-\clearpage
   \<^item> \<open>dt_ctor\<close>:\index{dt\_ctor@\<open>dt_ctor\<close>}
      \<^rail>\<open> name (type*) (mixfix?)\<close>
   \<^item> \<open>datatype_specification\<close>:\index{datatype\_specification@\<open>datatype_specification\<close>}
@@ -254,9 +253,9 @@ text\<open>
   \<^item> \<open>expr\<close>:\index{expr@\<open>expr\<close>}
      the syntactic category \<open>expr\<close> here denotes the very rich ``inner-syntax'' language of 
      mathematical  notations for $\lambda$-terms in Isabelle/HOL. Example expressions are:
-     \inlineisar|1+2| (arithmetics), \inlineisar|[1,2,3]| (lists), \inlineisar|''ab c''| (strings), 
-     \inlineisar|{1,2,3}| (sets), \inlineisar|(1,2,3)| (tuples), 
-     \inlineisar|\<forall> x. P(x) \<and> Q x = C| (formulas). For details, see~@{cite "nipkow:whats:2020"}.
+     \<^boxed_theory_text>\<open>1+2\<close> (arithmetics), \<^boxed_theory_text>\<open>[1,2,3]\<close> (lists), \<^boxed_theory_text>\<open>ab c\<close> (strings), 
+     \<^boxed_theory_text>\<open>{1,2,3}\<close> (sets), \<^boxed_theory_text>\<open>(1,2,3)\<close> (tuples), 
+     \<^boxed_theory_text>\<open>\<forall> x. P(x) \<and> Q x = C\<close> (formulas). For details, see~@{cite "nipkow:whats:2020"}.
 \<close>
 
 text\<open>
@@ -267,11 +266,11 @@ text\<open>
 
 text\<open>Note that \isadof works internally with fully qualified names in order to avoid 
 confusions occurring otherwise, for example, in disjoint class hierarchies. This also extends to 
-names for \inlineisar|doc_class|es, which must be representable as type-names as well since they
-can be used in attribute types. Since theory names are lexically very liberal (\inlineisar|0.thy|
-is a legal theory name), this can lead to subtle problems when constructing a class: \inlineisar|foo| 
-can be a legal name for a type definition, the corresponding type-name \inlineisar|0.foo| is not.
-For this reason, additional checks at the definition of a \inlineisar|doc_class| reject problematic
+names for \<^boxed_theory_text>\<open>doc_class\<close>es, which must be representable as type-names as well since they
+can be used in attribute types. Since theory names are lexically very liberal (\<^boxed_theory_text>\<open>0.thy\<close>
+is a legal theory name), this can lead to subtle problems when constructing a class: \<^boxed_theory_text>\<open>foo\<close> 
+can be a legal name for a type definition, the corresponding type-name \<^boxed_theory_text>\<open>0.foo\<close> is not.
+For this reason, additional checks at the definition of a \<^boxed_theory_text>\<open>doc_class\<close> reject problematic
 lexical overlaps.\<close>
 
 
@@ -310,7 +309,7 @@ text\<open>
   class-specific \LaTeX-definition can not only provide a specific layout (\eg, a specific 
   highlighting, printing of certain attributes), it can also generate entries in in the table of 
   contents or an index. Overall, the \inlineltx|\newisadof[]{}| command follows the structure
-  of the \inlineisar|doc_class|-command:
+  of the \<^boxed_theory_text>\<open>doc_class\<close>-command:
 
 \begin{ltx}[escapechar=ë]
 \newisadof{ë\<open>class_id\<close>ë}[label=,type=, ë\<open>attribute_decl\<close>ë][1]{%
@@ -324,7 +323,7 @@ text\<open>
   The \<open>class_id\<close> is the full-qualified name of the document class and the list of \<open>attribute_decl\<close>
   needs to declare all attributes of the document class. Within the \LaTeX-definition of the document
   class representation, the identifier \inlineltx|#1| refers to the content of the main text of the 
-  document class (written in \inlineisar|\<open> ... \<close>|) and the attributes can be referenced
+  document class (written in \<^boxed_theory_text>\<open>\<open> ... \<close>\<close>) and the attributes can be referenced
   by their name using the \inlineltx|\commandkey{...}|-command (see the documentation of the 
   \LaTeX-package ``keycommand''~@{cite "chervet:keycommand:2010"} for details). Usually, the 
   representations definition needs to be wrapped in a 
@@ -344,7 +343,7 @@ text\<open>
   Moreover, as usual, special care has to be taken for commands that write into aux-files
   that are included in a following \LaTeX-run. For such complex examples, we refer the interested 
   reader, in general, to  the style files provided in the \isadof distribution. In particular 
-  the definitions of the concepts \inlineisar|title*| and \inlineisar|author*| in the file 
+  the definitions of the concepts \<^boxed_theory_text>\<open>title*\<close> and \<^boxed_theory_text>\<open>author*\<close> in the file 
   \path{ontologies/scholarly_paper/DOF-scholarly_paper.sty} show examples of protecting special 
   characters in definitions that need to make use of a entries in an aux-file. 
 \<close>
@@ -352,7 +351,7 @@ text\<open>
 subsection\<open>Common Ontology Library (COL)\<close>
 
 text\<open>\isadof uses the concept of implicit abstract classes (or: \emph{shadow classes}).
-These refer to the set of possible \inlineisar+doc_class+ declarations that posses a number
+These refer to the set of possible \<^boxed_theory_text>\<open>doc_class\<close> declarations that posses a number
 of attributes with their types in common. Shadow classes represent an implicit requirement
 (or pre-condition) on a given class to posses these attributes in order to work properly
 for certain \isadof commands. 
@@ -387,7 +386,7 @@ text\<open>  \isadof provides a Common Ontology Library (COL)\index{Common Ontol
 
 
 text\<open>
-In particular it defines the super-class \inlineisar|text_element|: the
+In particular it defines the super-class \<^boxed_theory_text>\<open>text_element\<close>: the
   root of all text-elements,
 
 @{boxed_theory_text [display]\<open>
@@ -397,16 +396,16 @@ doc_class text_element =
    variants      :: "String.literal set" <= "{STR ''outline'', STR ''document''}" 
 \<close>}
 
-  Here, \inlineisar|level| defines the section-level (\eg, using a \LaTeX-inspired hierarchy:
-  from \inlineisar|Some -1| (corresponding to \inlineltx|\part|) to 
-  \inlineisar|Some 0| (corresponding to \inlineltx|\chapter|, respectively, \inlineisar|chapter*|) 
-  to \inlineisar|Some 3| (corresponding to \inlineltx|\subsubsection|, respectively, 
-  \inlineisar|subsubsection*|). Using an invariant, a derived ontology could, \eg, require that
+  Here, \<^boxed_theory_text>\<open>level\<close> defines the section-level (\eg, using a \LaTeX-inspired hierarchy:
+  from \<^boxed_theory_text>\<open>Some -1\<close> (corresponding to \inlineltx|\part|) to 
+  \<^boxed_theory_text>\<open>Some 0\<close> (corresponding to \inlineltx|\chapter|, respectively, \<^boxed_theory_text>\<open>chapter*\<close>) 
+  to \<^boxed_theory_text>\<open>Some 3\<close> (corresponding to \inlineltx|\subsubsection|, respectively, 
+  \<^boxed_theory_text>\<open>subsubsection*\<close>). Using an invariant, a derived ontology could, \eg, require that
   any sequence of technical-elements must be introduced by a text-element with a higher level
   (this would require that technical text section are introduce by a section element).
 
-Similarly, we provide "minimal" instances of the \inlineisar+ASSERTION_ALIKES+ 
-and \inlineisar+FORMAL_STATEMENT_ALIKE+ shadow classes:
+Similarly, we provide "minimal" instances of the \<^boxed_theory_text>\<open>ASSERTION_ALIKES\<close>
+and \<^boxed_theory_text>\<open>FORMAL_STATEMENT_ALIKE\<close> shadow classes:
 @{boxed_theory_text [display]\<open>
 doc_class assertions = 
     properties :: "term list"
@@ -436,9 +435,9 @@ doc_class EC = AC  +
   register the definition of ECs in a dedicated table of contents (\inlineltx{tos}) 
   and use an earlier defined environment \inlineltx|\begin{EC}...\end{EC}| for their graphical 
   representation. Note that the \inlineltx|\newisadof{}[]{}|-command requires the 
-  full-qualified names, \eg,  \inlineisar|t$$ext.CENELEC_50128.EC| for the document class and 
-  \inlineisar|CENELEC_50128.requirement.long_name| for the  attribute \inlineisar|long_name|, 
-  inherited from the document class \inlineisar|requirement|. The representation of ECs
+  full-qualified names, \eg,  \<^boxed_theory_text>\<open>text.CENELEC_50128.EC\<close> for the document class and 
+  \<^boxed_theory_text>\<open>CENELEC_50128.requirement.long_name\<close> for the  attribute \<^boxed_theory_text>\<open>long_name\<close>, 
+  inherited from the document class \<^boxed_theory_text>\<open>requirement\<close>. The representation of ECs
   can now be defined as follows:
 
 \begin{ltx}
@@ -493,18 +492,18 @@ assert*[claim::assertions] "last[1,2,3,4::int] = 4"
 \<close>}
 \<close>
 
-text\<open>As an \inlineisar+ASSERTION_ALIKES+, the \inlineisar+assertions+ class possesses a 
-\inlineisar+properties+ attribute. The \inlineisar+assert*+ command evaluates its argument;
-in case it evaluates to true the property is added to the property list of the \inlineisar+claim+ - 
-text-element. Commands like \inlineisar+Definitions*+ or \inlineisar+Theorem*+ work analogously.\<close>
+text\<open>As an \<^boxed_theory_text>\<open>ASSERTION_ALIKES\<close>, the \<^boxed_theory_text>\<open>assertions\<close> class possesses a 
+\<^boxed_theory_text>\<open>properties\<close> attribute. The \<^boxed_theory_text>\<open>assert*\<close> command evaluates its argument;
+in case it evaluates to true the property is added to the property list of the \<^boxed_theory_text>\<open>claim\<close> - 
+text-element. Commands like \<^boxed_theory_text>\<open>Definitions*\<close> or \<^boxed_theory_text>\<open>Theorem*\<close> work analogously.\<close>
 
 
 subsection*["text-elements"::technical]\<open>Annotatable Top-level Text-Elements\<close>
 text\<open>
   While the default user interface for class definitions via the  
-  \inlineisar|text*\<open> ... \<close>|-command allow to access all features of the document 
+  \<^boxed_theory_text>\<open>text*\<open> ... \<close>\<close>-command allow to access all features of the document 
   class, \isadof provides short-hands for certain, widely-used, concepts such as 
-  \inlineisar|title*\<open> ... \<close>| or \inlineisar|section*\<open> ... \<close>|, \eg:
+  \<^boxed_theory_text>\<open>title*\<open> ... \<close>\<close> or \<^boxed_theory_text>\<open>section*\<open> ... \<close>\<close>, \eg:
 
 @{boxed_theory_text [display]\<open>
  title*[title::title]\<open>Isabelle/DOF\<close>
@@ -554,10 +553,10 @@ text\<open>
   Defining such new top-level commands requires some Isabelle knowledge as well as 
   extending the dispatcher of the \LaTeX-backend. For the details of defining top-level 
   commands, we refer the reader to the Isar manual~@{cite "wenzel:isabelle-isar:2020"}. 
-  Here, we only give a brief example how the \inlineisar|section*|-command is defined; we 
+  Here, we only give a brief example how the \<^boxed_theory_text>\<open>section*\<close>-command is defined; we 
   refer the reader to the source code of \isadof for details.
 
-  First, new top-level keywords need to be declared in the \inlineisar|keywords|-section of 
+  First, new top-level keywords need to be declared in the \<^boxed_theory_text>\<open>keywords\<close>-section of 
   the theory header defining new keywords:
 
 @{boxed_theory_text [display]\<open>
@@ -632,24 +631,24 @@ text\<open>
   \<^emph>\<open>inside\<close> the HOL type system.  We do, however, not reflect the data of
   these types. They are just declared abstract types, 
   ``inhabited'' by special constant symbols carrying strings, for
-  example of the format \inlineisar+<@>{thm <string>}+. When HOL
-  expressions were used to denote values of \inlineisar+doc_class+
+  example of the format \<^boxed_theory_text>\<open>@{thm <string>}\<close>. When HOL
+  expressions were used to denote values of \<^boxed_theory_text>\<open>doc_class\<close>
   instance attributes, this requires additional checks after
   conventional type-checking that this string represents actually a
   defined entity in the context of the system state
-  \inlineisar+\<theta>+.  For example, the \inlineisar+establish+
+  \<^boxed_theory_text>\<open>\<theta>\<close>.  For example, the \<^boxed_theory_text>\<open>establish\<close>
   attribute in the previous section is the power of the ODL: here, we model
   a relation between \<^emph>\<open>claims\<close> and \<^emph>\<open>results\<close> which may be a
   formal, machine-check theorem of type \inlinesml+thm+ denoted by, for
-  example: \inlineisar+property = "[<@>{thm ''system_is_safe''}]"+ in a
-  system context \inlineisar+\<theta>+ where this theorem is
+  example: \<^boxed_theory_text>\<open>property = "[@{thm "system_is_safe"}]"\<close> in a
+  system context \<^boxed_theory_text>\<open>\<theta>\<close> where this theorem is
   established. Similarly, attribute values like 
-  \inlineisar+property = "<@>{term \<open>A \<leftrightarrow> B\<close>}"+
-  require that the HOL-string \inlineisar+A \<leftrightarrow> B+ is 
+  \<^boxed_theory_text>\<open>property = "@{term \<open>A \<leftrightarrow> B\<close>}"\<close>
+  require that the HOL-string \<^boxed_theory_text>\<open>A \<leftrightarrow> B\<close> is 
   again type-checked and represents indeed a formula in $\theta$. Another instance of 
   this process, which we call \<open>second-level type-checking\<close>, are term-constants
   generated from the ontology such as 
-  \inlineisar+<@>{definition <string>}+. 
+  \<^boxed_theory_text>\<open>@{definition <string>}\<close>. 
 \<close>
 
 
@@ -688,17 +687,17 @@ text\<open>
 text\<open>
   Monitored document sections can be nested and overlap; thus, it is
   possible to combine the effect of different monitors. For example, it
-  would be possible to refine the \inlineisar+example+ section by its own
+  would be possible to refine the \<^boxed_theory_text>\<open>example\<close> section by its own
   monitor and enforce a particular structure in the presentation of
   examples.
   
-  Monitors manage an implicit attribute \inlineisar+trace+ containing
+  Monitors manage an implicit attribute \<^boxed_theory_text>\<open>trace\<close> containing
   the list of ``observed'' text element instances belonging to the
   accept-set. Together with the concept of ODL class invariants, it is
   possible to specify properties of a sequence of instances occurring in
   the document section. For example, it is possible to express that in
-  the sub-list of \inlineisar+introduction+-elements, the first has an
-  \inlineisar+introduction+ element with a \inlineisar+level+ strictly
+  the sub-list of \<^boxed_theory_text>\<open>introduction\<close>-elements, the first has an
+  \<^boxed_theory_text>\<open>introduction\<close> element with a \<^boxed_theory_text>\<open>level\<close> strictly
   smaller than the others. Thus, an introduction is forced to have a
   header delimiting the borders of its representation. Class invariants
   on monitors allow for specifying structural properties on document
@@ -708,9 +707,9 @@ text\<open>
 subsubsection*["sec:class_inv"::technical]\<open>ODL Class Invariants\<close>
 text\<open>
   Ontological classes as described so far are too liberal in many situations. For example, one 
-  would like to express that any instance of a \inlineisar+result+ class finally has a non-empty 
-  property list, if its \inlineisar+kind+ is \inlineisar+p$$roof+, or that the \inlineisar+establish+ 
-  relation between \inlineisar+claim+ and \inlineisar+result+ is surjective.
+  would like to express that any instance of a \<^boxed_theory_text>\<open>result\<close> class finally has a non-empty 
+  property list, if its \<^boxed_theory_text>\<open>kind\<close> is \<^boxed_theory_text>\<open>proof\<close>, or that the \<^boxed_theory_text>\<open>establish\<close>
+  relation between \<^boxed_theory_text>\<open>claim\<close> and \<^boxed_theory_text>\<open>result\<close> is surjective.
 
   In a high-level syntax, this type of constraints could be expressed, \eg, by:
 
@@ -721,11 +720,11 @@ text\<open>
 (* 3 *) \<forall> x \<in> introduction. finite(x@authored_by)
 \<close>}
 
-  where \inlineisar+result+, \inlineisar+conclusion+, and \inlineisar+introduction+ are the set of
+  where \<^boxed_theory_text>\<open>result\<close>, \<^boxed_theory_text>\<open>conclusion\<close>, and \<^boxed_theory_text>\<open>introduction\<close> are the set of
   all possible instances of these document classes.  All specified constraints are already checked
   in the IDE of \dof while editing; it is however possible to delay a final error message till the 
   closing of a monitor (see next section). The third constraint enforces that the user sets the 
-  \inlineisar+authored_by+ set, otherwise an error will be reported.
+  \<^boxed_theory_text>\<open>authored_by\<close> set, otherwise an error will be reported.
 
   For the moment, there is no high-level syntax for the definition of class invariants. A 
   formulation, in SML, of the first class-invariant in \autoref{sec:class_inv} is straight-forward:
@@ -744,10 +743,10 @@ fun check_result_inv oid {is_monitor:bool} ctxt =
                                 "tiny_cert.result" check_result_inv)
 \end{sml}
 
-  The \inlinesml{setup}-command (last line) registers the \inlineisar+check_result_inv+ function 
+  The \inlinesml{setup}-command (last line) registers the \<^boxed_theory_text>\<open>check_result_inv\<close> function 
   into the \isadof kernel, which activates any creation or modification of an instance of 
-  \inlineisar+result+. We cannot replace \inlineisar+compute_attr_access+ by the corresponding 
-  antiquotation \inlineisar+<@>{docitem_value kind::oid}+, since \inlineisar+oid+ is bound to a 
+  \<^boxed_theory_text>\<open>result\<close>. We cannot replace \<^boxed_theory_text>\<open>compute_attr_access\<close> by the corresponding 
+  antiquotation \<^boxed_theory_text>\<open>@{docitem_value kind::oid}\<close>, since \<^boxed_theory_text>\<open>oid\<close> is bound to a 
   variable here and can therefore not be statically expanded.
 \<close>
 
@@ -896,7 +895,7 @@ text\<open>
 
 The new command \inlineltx|\addauthor| and a similarly defined command \inlineltx|\addaffiliation|
 can now be used in the definition of the representation of the concept 
-\inlineisar|text.scholarly_paper.author|, which writes the collected information in the 
+\<^boxed_theory_text>\<open>text.scholarly_paper.author\<close>, which writes the collected information in the 
 job's aux-file. The intermediate step of writing this information into the job's aux-file is necessary,
 as the author and affiliation information is required right at the begin of the document 
 (\ie, when \LaTeX's \inlineltx|\maketitle| is invoked) while  \isadof allows to define authors at 
@@ -962,10 +961,10 @@ text\<open>
   We encourage this clear and machine-checkable enforcement of restrictions while, at the same
   time, we also encourage to provide a package option to overwrite them. The latter allows 
   inherited ontologies to overwrite these restrictions and, therefore, to provide also support
-  for additional document templates. For example, the ontology \inlineisar|technical_report| 
-  extends the \inlineisar|scholarly_paper| ontology and its \LaTeX supports provides support
+  for additional document templates. For example, the ontology \<^boxed_theory_text>\<open>technical_report\<close>
+  extends the \<^boxed_theory_text>\<open>scholarly_paper\<close> ontology and its \LaTeX supports provides support
   for the \inlineltx|scrrept|-class which is not supported by the \LaTeX support for 
-  \inlineisar|scholarly_paper|.
+  \<^boxed_theory_text>\<open>scholarly_paper\<close>.
 \<close>
 
 subsubsection\<open>Outdated Version of \path{comment.sty}\<close>
